pre abstract machine generation, staged abstract machine sig

refocusing_signatures.v
@@ -83,6 +83,7 @@ Module Type RED_REF_SEM (R : RED_LANG).
                dec_term t k2 = in_term t0 ec ->
                dec t0 (ec=:c) d ->
                dec t c d
+
   with decctx : forall {k2}, value k2 -> forall {k1}, context k1 k2 -> decomp k1 -> Prop :=
   | dc_end  : forall {k} (v : value k), 
                 ~ dead_ckind k ->
@@ -102,11 +103,14 @@ Module Type RED_REF_SEM (R : RED_LANG).
                 decctx v (ec=:c) d.
 
   Scheme dec_Ind := Induction for dec Sort Prop
-   with decctx_Ind := Induction for decctx Sort Prop.
+    with decctx_Ind := Induction for decctx Sort Prop.
 
 
   Axiom dec_val_self : forall {k2} (v : value k2) {k1} {c : context k1 k2} {d}, 
                            dec v c d <-> decctx v c d.
+
+  Axiom dec_not_dead : forall {t k1 k2} {c : context k1 k2} {d},
+                           dec t c d -> ~ dead_ckind k2.
 
   Declare Module RS : RED_SEM R with Definition dec := dec.
 
@@ -153,3 +157,144 @@ Module Type RED_SEM_PROPER (R : RED_LANG) (RS : RED_SEM R).
                   t = c'[r'] -> k2' = k2 /\ r ~= r' /\ c ~= c').
 
 End RED_SEM_PROPER.
+
+
+
+Module Type PRE_ABSTRACT_MACHINE (R : RED_LANG).
+
+  Import R.
+
+  (** Functions specifying atomic steps of induction on terms and contexts -- needed to avoid explicit induction on terms and contexts in construction of the AM *)
+  Parameter dec_term    : term -> forall k, interm_dec k.
+  Parameter dec_context : forall ec k, value (k+>ec) -> interm_dec k.
+
+  Axiom dec_term_correct : 
+      forall t k, match dec_term t k with
+      | in_red r       => t = r
+      | in_val v       => t = v
+      | in_term t0 ec0 => t = ec0:[t0]
+      | in_dead        => dead_ckind k
+      end.
+
+  Axiom dec_context_correct : 
+      forall ec k v, match dec_context ec k v with
+      | in_red r      => ec:[v] = r
+      | in_val v0     => ec:[v] = v0
+      | in_term t ec0 => ec:[v] = ec0:[t]
+      | in_dead       => dead_ckind (k+>ec) 
+      end.
+  
+  (** A decomposition function specified in terms of the atomic functions above *)
+  Inductive dec : term -> forall {k1 k2}, context k1 k2 -> decomp k1 -> Prop :=
+  | d_dec  : forall t {k1 k2} (c : context k1 k2) {r},
+               dec_term t k2 = in_red r -> 
+               dec t c (d_red r c)
+  | d_v    : forall t {k1 k2} {c : context k1 k2} {v d},
+               dec_term t k2 = in_val v ->
+               decctx v c d ->
+               dec t c d
+  | d_term : forall t {t0 k1 k2} {c : context k1 k2} {ec d},
+               dec_term t k2 = in_term t0 ec ->
+               dec t0 (ec=:c) d ->
+               dec t c d
+
+  with decctx : forall {k2}, value k2 -> forall {k1}, context k1 k2 -> decomp k1 -> Prop :=
+  | dc_end  : forall {k} (v : value k), 
+                ~ dead_ckind k ->
+                decctx v [_] (d_val v)
+  | dc_dec  : forall ec {k2} (v : value (k2+>ec)) {k1} (c : context k1 k2) {r},
+                dec_context ec k2 v = in_red r ->
+                decctx v (ec=:c) (d_red r c)
+  | dc_val  : forall {k2} {v0 : value k2} ec (v : value (k2+>ec)) 
+                     {k1} {c  : context k1 k2} {d},
+                dec_context ec k2 v = in_val v0 ->
+                decctx v0 c d ->
+                decctx v (ec=:c) d
+  | dc_term : forall ec {ec0 k2} (v : value (k2+>ec)) 
+                            {k1} {c : context k1 k2} {t d},
+                dec_context ec k2 v = in_term t ec0 ->
+                dec t (ec0=:c) d ->
+                decctx v (ec=:c) d.
+
+  Scheme dec_Ind := Induction for dec Sort Prop
+    with decctx_Ind := Induction for decctx Sort Prop.
+
+  Inductive iter : forall {k}, decomp k -> value k -> Prop :=
+  | i_val : forall {k} (v : value k), iter (d_val v) v
+  | i_red : forall {k2} (r : redex k2) {t k1} {c : context k1 k2} {d v},
+              contract r = Some t -> dec t c d -> iter d v ->
+              iter (d_red r c) v.
+
+  Inductive eval : term -> forall {k}, value k -> Prop :=
+  | e_intro : forall {t k} {d : decomp k} {v},
+                dec t [_] d -> iter d v -> eval t v.
+
+End PRE_ABSTRACT_MACHINE.
+
+
+
+Module Type STAGED_ABSTRACT_MACHINE (R : RED_LANG).
+
+  Import R.
+
+  (** Functions specifying atomic steps of induction on terms and contexts -- needed to avoid explicit induction on terms and contexts in construction of the AM *)
+  Parameter dec_term    : term -> forall k, interm_dec k.
+  Parameter dec_context : forall ec k, value (k+>ec) -> interm_dec k.
+
+  Axiom dec_term_correct : 
+      forall t k, match dec_term t k with
+      | in_red r       => t = r
+      | in_val v       => t = v
+      | in_term t0 ec0 => t = ec0:[t0]
+      | in_dead        => dead_ckind k
+      end.
+
+  Axiom dec_context_correct : 
+      forall ec k v, match dec_context ec k v with
+      | in_red r      => ec:[v] = r
+      | in_val v0     => ec:[v] = v0
+      | in_term t ec0 => ec:[v] = ec0:[t]
+      | in_dead       => dead_ckind (k+>ec) 
+      end.
+
+
+  Inductive dec : term -> forall {k1 k2}, context k1 k2 -> value k1 -> Prop :=
+  | d_dec  : forall t {k1 k2} {c : context k1 k2} {r v},
+               dec_term t k2 = in_red r -> iter (d_red r c) v ->
+               dec t c v
+  | d_v    : forall t {k1 k2} {c : context k1 k2} {v v0},
+               dec_term t k2 = in_val v -> decctx v c v0 ->
+               dec t c v0
+  | d_many : forall t {t0 ec k1 k2} {c : context k1 k2} {v},
+               dec_term t k2 = in_term t0 ec -> dec t0 (ec=:c) v ->
+               dec t c v
+
+  with decctx : forall {k2}, value k2 -> forall {k1}, context k1 k2 -> value k1 -> Prop :=
+  | dc_end  : forall {k} {v v0 : value k},
+               iter (d_val v) v0 ->
+               decctx v [_] v0
+  | dc_dec  : forall ec {k2} (v : value (k2+>ec)) {k1} {c : context k1 k2} {r v0},
+               dec_context ec k2 v = in_red r -> iter (d_red r c) v0 ->
+               decctx v (ec=:c) v0
+  | dc_val  : forall ec {k2} (v : value (k2+>ec)) {v0 k1} {c : context k1 k2} {v1},
+               dec_context ec k2 v = in_val v0 -> decctx v0 c v1 ->
+               decctx v (ec=:c) v1
+  | dc_term : forall ec {k2} (v : value (k2+>ec)) {t ec0 k1} {c : context k1 k2} {v0},
+               dec_context ec k2 v = in_term t ec0 -> dec t (ec0=:c) v0 ->
+               decctx v (ec=:c) v0
+
+  with iter : forall {k}, decomp k -> value k -> Prop :=
+  | i_val : forall {k} (v : value k), 
+               iter (d_val v) v
+  | i_red : forall {k2} (r : redex k2) {k1} {c : context k1 k2} {t v},
+               contract r = Some t -> dec t c v -> 
+               iter (d_red r c) v.
+
+  Scheme dec_Ind    := Induction for dec Sort Prop
+    with decctx_Ind := Induction for decctx Sort Prop
+    with iter_Ind   := Induction for iter Sort Prop.
+
+  Inductive eval : term -> forall {k}, value k -> Prop :=
+  | e_intro : forall {t k} {v : value k}, dec t [_] v -> eval t v.
+
+End STAGED_ABSTRACT_MACHINE.
